More updates on example code

src/IfExp/Syntax.hs
@@ -1,0 +1,78 @@
+module IfExp.Syntax where 
+
+data IExp 
+  = IZero 
+  | ISucc IExp 
+  | IIsZero IExp 
+  | IPred IExp 
+  | ITrue 
+  | IFalse 
+  | IIf IExp IExp IExp 
+  deriving (Eq, Show)
+
+interp :: IExp -> Result Value 
+interp IZero = pure (Right NZero)
+interp ITrue = pure (Left BTrue)
+interp IFalse = pure (Left BFalse)
+interp (ISucc e) 
+  = do 
+      v <- interp e 
+      case v of 
+        Right nv -> pure (Right (NSucc nv))
+        _        -> TypeError 
+interp (IPred e)
+  = do 
+      v <- interp e 
+      case v of 
+        Left _ -> TypeError 
+        Right NZero -> pure (Right NZero)
+        Right (NSucc nv) -> pure (Right nv)
+interp (IIsZero e)
+  = do 
+      v <- interp e 
+      case v of 
+        Left _ -> TypeError 
+        Right NZero -> pure (Left BTrue)
+        Right (NSucc _) -> pure (Left BFalse)
+interp (IIf e1 e2 e3) 
+  = do 
+      v1 <- interp e1 
+      case v1 of 
+        Right _ -> TypeError 
+        Left BTrue -> interp e2 
+        Left BFalse -> interp e3 
+
+
+type Value = Either BValue NValue 
+
+data BValue 
+  = BTrue 
+  | BFalse 
+  deriving (Eq, Show)
+
+data NValue 
+  = NZero 
+  | NSucc NValue 
+  deriving (Eq, Show)
+
+data Result a 
+  = Ok a 
+  | TypeError 
+  deriving (Eq, Show) 
+
+instance Functor Result where 
+  fmap f (Ok v) = Ok (f v)
+  fmap _ TypeError = TypeError 
+
+instance Applicative Result where 
+  pure = Ok 
+  (Ok f) <*> (Ok x) = Ok (f x)
+  TypeError <*> _ = TypeError 
+  _ <*> TypeError = TypeError
+
+instance Monad Result where 
+  return = pure 
+  (Ok m) >>= f = f m 
+  TypeError >>= _ = TypeError 
+
+
