src/Parser/Common/ExtendGrammar.hs
@@ -1,0 +1,42 @@
+module Parser.Common.ExtendGrammar where 
+
+import Data.List ((\\))
+import Parser.Common.Grammar 
+
+-- creating the extended grammar by adding 
+-- a new production
+
+extendGrammar :: Grammar -> Grammar 
+extendGrammar g = Grammar rules' n' 
+  where 
+    n' = freshNT g 
+    rules' = [ n' +-> [Symb Dot, Var (start g), Symb Dollar ]] ++ 
+             productions g
+
+-- creating a list of fresh non-terminals
+
+freshNT :: Grammar -> Nonterminal 
+freshNT g = NT v 
+  where 
+    (v, _) = deplete (ntPool \\ ns) 
+    ns = ntName <$> nonterminals g 
+
+ntName :: Nonterminal -> String 
+ntName (NT s) = s
+
+deplete :: [String] -> (String, [String])
+deplete (x : xs) = (x, xs)
+deplete [] = ("", [])
+
+ntPool :: [String]
+ntPool 
+  = names ++ addNumber names ([1..] :: [Int])
+  where 
+    wrap x = [x]
+    names = map wrap ['A' .. 'Z']
+    addNumber :: [String] -> [Int] -> [String]
+    addNumber as bs = do 
+      a <- as 
+      b <- bs 
+      return $ a ++ show b
+
