src/Parser/Common/Table.hs
@@ -1,0 +1,26 @@
+module Parser.Common.Table ( Table
+                           , toTableString
+                           ) where
+
+import Data.Map (Map)
+import qualified Data.Map as Map
+
+import Parser.Common.Grammar
+
+
+type Table = Map (Nonterminal, Terminal) [Production]
+
+toTableString :: Table -> String
+toTableString tbl
+  = concatMap format (Map.toList tbl)
+    where
+      format ((nt, t), p) = concat [ "M["
+                                   , show nt
+                                   , ", "
+                                   , show t
+                                   , "] = "
+                                   , show p
+                                   , "\n"
+                                   ]
+
+
