src/Parser/LR/LR0/MkLR0Table.hs
@@ -1,0 +1,51 @@
+module Parser.LR.LR0.MkLR0Table where 
+
+import Control.Monad.State 
+import Control.Monad.Except 
+
+import Data.List 
+import Data.Map (Map)
+import qualified Data.Map as Map 
+
+import Parser.Common.ExtendGrammar
+import Parser.Common.Grammar
+
+-- definition of the table 
+
+type Table = Map (Int, Symbol) (Action, Item)
+
+-- type of Action 
+
+data Action 
+  = Shift Symbol 
+  | Reduce Production 
+  | Error 
+  | Accept 
+  deriving Eq 
+
+instance Show Action where 
+  show (Shift s) = "Shift: " ++ show s 
+  show (Reduce r) = "Reduce: " ++ show r 
+  show Error = "Error"
+  show Accept = "Accept"
+
+-- definition of an item 
+
+type Item 
+  = [Production]
+
+-- definition of the monad 
+
+data Env 
+  = Env {
+      fresh :: Int
+    , states :: [Item]
+    , table :: Table 
+    }
+
+type TableM a = StateT Env (ExceptT String IO) a
+
+-- auxiliar stuff 
+
+subset :: Eq a => [a] -> [a] -> Bool 
+subset xs ys = all (\ x -> x `elem` ys) xs
