lean/Imp/Hoare.lean
@@ -7,9 +7,13 @@ import Imp.Syntax
 import Imp.Interpreter 
 import Imp.Semantics 
 
+-- assertions 
+
+abbrev Assertion := Env → Prop 
+
 -- Hoare logic 
 
-def Hoare (P : Env → Prop)(s : Stmt)(Q : Env → Prop) :=
+def Hoare (P : Assertion)(s : Stmt)(Q : Assertion) :=
   ∀ (env env' : Env), P env → Eval env s env' → Q env'
 
 macro "{*" P:term " *} " "(" s:term ")" " {* " Q:term " *}" : term =>
@@ -17,7 +21,7 @@ macro "{*" P:term " *} " "(" s:term ")" " {* " Q:term " *}" : term =>
 
 -- rules of Hoare logic 
 
-theorem Skip_rule (P : Env → Prop) 
+theorem Skip_rule (P : Assertion) 
   : {* P *} (Stmt.Skip) {* P *}:= by 
   intros env env' Hp Hev
   cases Hev 
@@ -25,13 +29,13 @@ theorem Skip_rule (P : Env → Prop)
 
 def assertion_sub (s : String) 
                   (e : IExp) 
-                  (P : Env → Prop) : Env → Prop := 
+                  (P : Assertion) : Assertion := 
   λ env => P (s |-> (evalExp e env) ; env)
 
 macro P:term "[*" s:term "↦" e:term "*]" : term => 
   `(assertion_sub $s $e $P)
 
-theorem Assign_rule (P : Env → Prop)
+theorem Assign_rule (P : Assertion)
   s e :   {* P [* s ↦ e *] *}
             (Stmt.Assign s e) 
           {* P *} := by 
@@ -42,10 +46,60 @@ theorem Assign_rule (P : Env → Prop)
   rw [← He]
   assumption
 
-theorem Seq_rule (P Q R : Env → Prop) s1 s2 
+theorem Seq_rule (P Q R : Assertion) s1 s2 
   : {* P *} (s1) {* Q *} → 
     {* Q *} (s2) {* R *} → 
     {* P *} (.Seq s1 s2) {* R *} := by
     intros H1 H2 env env' HP Hs 
-    rcases Hs ; aesop 
+    rcases Hs ; aesop
 
+macro P:term "∧ True(" b:term ")" : term => 
+  `(λ st => $P st ∧ evalExp $b st > 0)
+
+macro P:term "∧ False(" b:term ")" : term => 
+  `(λ st => $P st ∧ evalExp $b st = 0)
+
+theorem If_rule (P Q : Assertion) b s1 s2 
+  : {* P ∧ True(b) *} (s1) {* Q *} → 
+    {* P ∧ False(b) *} (s2) {* Q *} → 
+    {* P *} (.If b s1 s2) {* Q *} := by 
+    intros H1 H2 
+    intros env env' HPenv HEval 
+    rcases HEval 
+    · 
+      rename_i v Hb Henv' 
+      apply H1 <;> aesop
+    · 
+      rename_i H3 H4 
+      apply H2 <;> aesop
+
+
+theorem While_rule (P : Assertion) b s 
+  : {* P ∧ True(b) *} (s) {* P *} → 
+    {* P *} (.While b s) {* P ∧ False(b) *} := by 
+    intros H1 env env' Hp HEval
+    have H2 : ∃ x, x = Stmt.While b s := by 
+      exists (Stmt.While b s)
+    rcases H2 with ⟨ v , Heq ⟩ 
+    rw [← Heq] at HEval 
+    induction' HEval <;> try rcases Heq 
+    · 
+      rename_i env' H1
+      aesop 
+    · 
+      rename_i env0 env1 env2 v Hexp Heval _IH2 _Heval1 IH1
+      apply IH1 
+      apply H1
+      · 
+        constructor 
+        · 
+          exact Hp
+        · 
+          rw [Hexp]
+          simp 
+      · 
+        exact Heval 
+      · 
+        rfl 
+
+    
